about to use his theta instead of mine

trans.v
@@ -1,12 +1,17 @@
 From istari Require Import Sigma Tactics
      Syntax Subst SimpSub Promote Hygiene
-     ContextHygiene Equivalence Rules.
+     ContextHygiene Equivalence Rules Defined.
+
+Definition oof (M: term False) := deq M M.
 
 Definition plus L R : (term False) := sigma booltp (bite (var 0) (subst (sh 1) L)
                                            (subst (sh 1) R) ).
 Definition inl L: term False := ppair btrue L.
 Definition inr R: term False := ppair bfalse R.
 
+Definition opt w: term False := sigma booltp (bite (var 0) w unittp).
+
+(*recursion*)
 Definition theta : (term False) :=
   lam(
       lam (
@@ -54,4 +59,81 @@ Definition bind : term False := app Yc
                let f' := prev f in
                inr (next (app (app f' y') g))) )
         ))).
+(*worlds*)
 
+ Definition list: (term False) -> (term False) := fun A => wt (opt A) (bite (ppi1 (var 0)) unittp voidtp).
+
+ Definition cons: (term False) -> (term False) -> (term False) := fun x => fun L => ppair (ppair btrue x)
+                                                                      (lam L).
+
+ Definition hd: (term False) -> (term False) := fun L => ppi2 (ppi1 L).
+
+ Definition tl: (term False) -> (term False) := fun L => (app (ppi2 L) triv).
+
+ Definition if_cons: (term False) -> (term False) := fun L => ppi1 (ppi1 L).
+
+ Definition one: (term False) := nsucc nzero.
+
+ Definition world: (term False) := rec (list (karrow (fut (var 0)) (univ (one)))).
+
+ Definition tlist: (term False) := list (univ one).
+
+ Definition app_bc: (term False) := lam 
+                      ( (*f:= 0*)
+                         lam ( (*f:= 1; L1 := 0*)
+                               lam ( (*f := 2; L1 := 1; L2 := 0*)
+                                     let f := (var 2) in
+                                     let L1 := (var 1) in
+                                     let L2 := (var 0) in
+bite (if_cons L1) (cons (hd L1) (app (app f (tl L1)) L2 )) L2
+)
+)
+).
+
+ Definition pend: (term False) := app (app theta theta) app_bc.
+
+ Definition subseq: (term False) -> (term False) -> (term False) :=
+   fun w1 => fun w2 => exist one world (equal w2 (app (app pend (var 0)) w1)
+                                                              world).
+
+ Lemma osub : forall (M M' U1 U2 U3: term False) (G: context),
+                         tr G (oof M (subseq U2 U3))
+                         -> tr G (oof M' (subseq U1 U2))
+                         ->tr G (oof triv (subseq U1 U3)).
+ Admitted.
+
+ Definition getstorebc: (term False) := lam
+                                      ( (*f := var 0*)
+                         lam  ((*f := 1, w := 0*)
+                             lam ( (*f:= 2, w:= 1, v:= 0*)
+                                 let f := var 2 in
+                                 let w := var 1 in
+                                 let v := var 0 in
+bite (if_cons w) (cons (app (hd w) (next v)) (app (app f (tl w)) v)) unittp
+)
+)
+                                      ).
+ (** getstore w v ~:= * (w/v) *)
+
+ Definition getstore: (term False) := app (app theta theta) getstorebc.
+
+ Definition store: (term False) -> (term False) := fun w => all one world ( (*u := var 0*)
+                                                  pi 
+                                                    (subseq w (var 0))
+                                                    (*u :=  var 1, m := var 0*)
+                                                     (app (app getstore w) (var 1))
+).
+
+ (*nats*)
+ Definition minusbc: (term False) := lam 
+                         (
+                           (*f := 0*)
+                           lam ( (*f:= 1, n := 0*)
+                                       lam ((*f := 2, n:= 1, m := 0*)
+                                                  bite (if_z n)
+                                                  (nzero)
+                                                  (bite (if_z m)
+                                                     (n)
+                                                    (app (app f (app (ppi2 n) triv)) (app (ppi2 m) triv)))
+                                                  ))).
+ Definition minus: (term False) := app (app theta theta) minusbc.
